### Steps 

- derive a recursive T(n) equation
- we use recursion tree method
- - we write non-recursive part as root of tree and recursive part as children
- - we keep expanding children until we see a pattern 


### Q) find order of growth of the below code

```

1)  void fun(int n)
    {
        if( n <= 1)
            return;
        print("heylo!!")
        fun(n/2)
        fun(n/2)
    }

Ans: Let's assume fun(n) function has some T(n) complexity 
hence fun(n/2) will have T(n/2) complexity

T(n) = time complexity of fun(n/2) + time complexity of fun(n/2) + time complexity of print statement
T(n)   = 2T(n/2) + k 
for base case, n = 1, T(1) = c

2)  void fun(int n)
    {
        if( n <= 1)
            return;
        print(n)
        fun(n-1)
    }

Ans: Let's assume fun(n) function has some T(n) complexity 
hence fun(n-1) will have T(n-1) complexity

T(n) = time complexity of fun(n-1) + time complexity of print statement
T(n)  = T(n-1) + k 
for base case, n = 1, T(1) = c


3)  void fun(int n)
    {
        if( n <= 1)
            return;
        for(int i = 0; i < n; i++)
            printf("Bye World");
        fun(n/2)
        fun(n/2)
    }

Ans: Let's assume fun(n) function has some T(n) complexity 
hence fun(n/2) will have T(n/2) complexity

T(n) = time complexity of fun(n/2) + time complexity of fun(n/2) + time complexity of for-loop
     = 2T(n/2) + O(n)

for base case, n = 1, T(1) = c
